theory/math.dfy
@@ -239,34 +239,38 @@ ghost function {:axiom} ceil(x:real) : int
 
 type R0 = r | r >= 0.0 witness 0.0
 
-ghost function powr0(x:R0, y:R0) : R0
+ghost function {:axiom} powr(x:real, y:real) : real
+  ensures x >= 0.0 && y >= 0.0 ==> powr(x, y) >= 0.0  
 
-lemma {:axiom} lem_powrZero(x:R0)
+lemma {:axiom} lem_powrZeroZero() // assume 0.0^0.0 = 1
+  ensures  powr(0.0, 0.0) == 1.0 
+
+lemma {:axiom} lem_powrZero(x:real)
   requires x > 0.0
-  ensures  powr0(x, 0.0) == 1.0 
+  ensures  powr(x, 0.0) == 1.0 
 
-lemma {:axiom} lem_powrOne(x:R0)
+lemma {:axiom} lem_powrOne(x:real)
   requires x > 0.0
-  ensures  powr0(x, 1.0) == x
+  ensures  powr(x, 1.0) == x
 
-lemma {:axiom} lem_powrProduct(x:R0, y:R0, z:R0)
+lemma {:axiom} lem_powrProduct(x:real, y:real, z:real)
   requires x > 0.0 
-  ensures powr0(x, y+z) == powr0(x, y)*powr0(x, z)  
+  ensures powr(x, y+z) == powr(x, y)*powr(x, z)  
 
 lemma {:axiom} lem_powrZeroAll()
-  ensures forall x:R0 :: x > 0.0 ==> powr0(x, 0.0) == 1.0 
+  ensures forall x:real :: x > 0.0 ==> powr(x, 0.0) == 1.0 
 
 lemma {:axiom} lem_powrOneAll()
-  ensures forall x:R0 :: x > 0.0 ==> powr0(x, 1.0) == x  
+  ensures forall x:real :: x > 0.0 ==> powr(x, 1.0) == x  
 
 lemma {:axiom} lem_powrProductAll()
-  ensures forall x:R0, y:R0, z:R0 :: x > 0.0 ==> powr0(x, y+z) == powr0(x, y)*powr0(x, z)
+  ensures forall x:real, y:real, z:real :: x > 0.0 ==> powr(x, y+z) == powr(x, y)*powr(x, z)
 
-lemma lem_powrTwo(x:R0) 
+lemma lem_powrTwo(x:real) 
   requires x > 0.0
-  ensures powr0(x, 2.0) == x*x
+  ensures powr(x, 2.0) == x*x
 {  
-  assert powr0(x, 2.0) == powr0(x, 1.0 + 1.0);
+  assert powr(x, 2.0) == powr(x, 1.0 + 1.0);
   lem_powrProduct(x, 1.0, 1.0);
   lem_powrOne(x);
 } 
@@ -284,122 +288,197 @@ lemma {:axiom} lem_funExt<A,B>(f1:A->B, f2:A->B)
 **************************************************************************/
 
 // sum_{k=i}^{j}f(k)
-opaque ghost function sum(i:nat, j:nat, f:nat->nat): nat
+opaque ghost function sumr(i:int, j:int, f:int->real): real
   decreases j - i
 {
   if i > j  
-  then 0 
-  else f(i) + sum(i+1 , j, f)
+  then 0.0
+  else f(i) + sumr(i+1 , j, f)
 }
 
-// i <= j+1 ==>   sum_{k=i}^{j}ITE(i<=k<=j,f(k),0) 
-//              = f(i) + sum_{k=i+1}^{j}ITE(i+1<=k<=j,f(k),0)
-lemma {:axiom} lem_sumGuardedDropFirst(i:nat, j:nat, f:nat->nat)
-  requires i <= j+1
-  ensures    sum(i, j, k => if i<=k<=j then f(k) else 0) 
-          ==   (if i<=i<=j then f(i) else 0) 
-             + sum(i+1, j, k => if i+1<=k<=j then f(k) else 0) 
-
-lemma {:axiom} lem_sumGuardedShiftLowerBound(i:nat, j:nat, f:nat->nat)
-  //requires i+1 <= j
-  ensures    sum(i+1, j, k => if i+1<=k<=j then f(k) else 0) 
-          == sum(i+1, j, k => if i<=k<=j then f(k) else 0) 
-
 // i <= j+1 ==> sum_{k=i}^{j+1}f(k) = sum_{k=i}^{j}f(k) + f(j+1)
-lemma lem_sumDropLast(i:nat, j:nat, f:nat->nat)
+lemma lem_sumrDropLast(i:int, j:int, f:int->real)
   requires i <= j+1
   decreases j - i
-  ensures sum(i, j+1, f) == sum(i, j, f) + f(j+1) 
+  ensures sumr(i, j+1, f) == sumr(i, j, f) + f(j+1) 
 { 
   if i == j+1 {   
     // BC: i > j
     calc {
-         sum(j+1, j+1, f);
-      == { reveal sum(); }
+         sumr(j+1, j+1, f);
+      == { reveal sumr(); }
          f(j+1);
       == 
-         0 + f(j+1) ;
-      == { reveal sum(); }
-         sum(i, j, f) + f(j+1) ;       
+         0.0 + f(j+1) ;
+      == { reveal sumr(); }
+         sumr(i, j, f) + f(j+1) ;       
     }
   } else {  
     // Step. i <= j
     //   IH: sum(i+1, j+1, f) = sum(i+1, j, f) + f(j+1)
     //    T: sum(i, j+1, f)   = sum(i, j, f)   + f(j+1)
     calc {  
-         sum(i, j+1, f);
-      == { reveal sum(); } 
-         f(i) + sum(i+1, j+1, f);
-      == { lem_sumDropLast(i+1, j, f); }  // by IH
-         f(i) + (sum(i+1, j, f) + f(j+1));
+         sumr(i, j+1, f);
+      == { reveal sumr(); } 
+         f(i) + sumr(i+1, j+1, f);
+      == { lem_sumrDropLast(i+1, j, f); }  // by IH
+         f(i) + (sumr(i+1, j, f) + f(j+1));
       == 
-         (f(i) + sum(i+1, j, f)) + f(j+1);
-      == { reveal sum(); }
-         sum(i, j, f) + f(j+1);           
+         (f(i) + sumr(i+1, j, f)) + f(j+1);
+      == { reveal sumr(); }
+         sumr(i, j, f) + f(j+1);           
     }
   }
 } 
 
-lemma lem_sumDropLastAll(i:nat, j:nat)
+lemma lem_sumrDropLastAll(i:int, j:int)
   requires i <= j+1
-  ensures forall f:nat->nat :: sum(i, j+1, f) == sum(i, j, f) + f(j+1) 
+  ensures forall f:int->real :: sumr(i, j+1, f) == sumr(i, j, f) + f(j+1) 
 { 
-  forall f:nat->nat
-    ensures sum(i, j+1, f) == sum(i, j, f) + f(j+1) 
+  forall f:int->real
+    ensures sumr(i, j+1, f) == sumr(i, j, f) + f(j+1) 
   {
-     lem_sumDropLast(i, j, f);
+     lem_sumrDropLast(i, j, f);
   }
-} 
+}
 
 // i <= j+1 ==> sum_{k=i}^{j}c = c*(j - i + 1)
-lemma lem_sumOverConst(i:nat, j:nat, c:nat)
+lemma lem_sumrOverConst(i:int, j:int, c:real)
   requires i <= j+1
   decreases j - i
-  ensures sum(i, j, k => c) == c*(j - i + 1)
+  ensures sumr(i, j, k => c) == c * (j - i + 1) as real
 { 
   if i == j+1 {   
     // BC: i > j
     calc {
-         sum(j+1, j, k => c);
-      == { reveal sum(); }
-         0;
-      == 
-         j - (j+1) + 1;
+         sumr(j+1, j, k => c); 
+      == { reveal sumr(); } 
+         0.0; 
+      == (j - (j+1) + 1) as real;
     }
   } else {  
     // Step. i <= j
     //   IH: sum(i+1, j, k => c) = c*(j -(i+1) + 1) = c*(j - i)
     //    T: sum(i, j, k => c)   = c*(j -i + 1) 
     calc {  
-         sum(i, j, k => c);
-      == { reveal sum(); }
-         c + sum(i+1, j, x => c);
-      == { lem_sumOverConst(i+1, j, c); }  // by IH
-         c + c*(j -(i+1) + 1);
+         sumr(i, j, k => c);
+      == { reveal sumr(); }
+         c + sumr(i+1, j, x => c);
+      == { lem_sumrOverConst(i+1, j, c); }  // by IH
+         (c + c* (j -(i+1) + 1) as real);
       == 
-         c + c*(j - i);      
+         c + c*((j - i) as real) ;      
       == 
-         c*(j -i + 1);             
+         c* (j -i + 1) as real;             
     }
   }
 }
 
-lemma lem_sumOverConstAll(i:nat, j:nat)
+lemma lem_sumrOverConstAll(i:int, j:int)
   requires i <= j+1
-  ensures forall c:nat :: sum(i, j, x => c) == c*(j - i + 1)
+  ensures forall c:real :: sumr(i, j, k => c) == c * (j - i + 1) as real
 { 
-  forall c:nat
-    ensures sum(i, j, x => c) == c*(j - i + 1)
+  forall c:real
+    ensures sumr(i, j, k => c) == c * (j - i + 1) as real
+  {
+     lem_sumrOverConst(i, j, c);
+  }
+} 
+
+// i <= j+1 /\ (∀ k : i<=k<=j : f(k) == g(k)) 
+//          ==> sum_{k=i}^{j}f = sum_{k=i}^{j}g
+lemma {:axiom} lem_sumrLeibniz(i:int, j:int, f:int->real, g:int->real)
+  requires i <= j+1
+  requires forall k:int :: i<=k<=j ==> f(k) == g(k)
+  ensures sumr(i, j, f) == sumr(i, j, g)
+
+
+/**************************************************************************
+  A special version of Sum over intervals on integer codomain
+**************************************************************************/
+ 
+// sum_{k=i}^{j}f(k)
+opaque ghost function sum(i:int, j:int, f:int->int) : int
+  decreases j - i
+{
+  if i > j  
+  then 0
+  else f(i) + sum(i+1, j, f)
+}
+
+lemma lem_sum_liftCi2r_eq(i:int, j:int, f:int->int)
+  requires i <= j+1
+  decreases j - i
+  ensures sumr(i, j, liftCi2r(f)) == sum(i, j, f) as real
+{
+  reveal sum(), sumr();
+}  
+
+// i <= j+1 ==> sum_{k=i}^{j+1}f(k) = sum_{k=i}^{j}f(k) + f(j+1)
+lemma lem_sumDropLast(i:int, j:int, f:int->int)
+  requires i <= j+1
+  ensures sum(i, j+1, f) == sum(i, j, f) + f(j+1) 
+{ 
+  var fr := liftCi2r(f);
+  lem_sumrDropLast(i, j, fr);
+  assert sumr(i, j+1, fr) == sumr(i, j, fr) + fr(j+1);
+  lem_sum_liftCi2r_eq(i, j+1, f);
+  lem_sum_liftCi2r_eq(i, j, f);
+}
+
+lemma lem_sumDropLastAll(i:int, j:int)
+  requires i <= j+1
+  ensures forall f:int->int :: sum(i, j+1, f) == sum(i, j, f) + f(j+1) 
+{ 
+  forall f:int->int
+    ensures sum(i, j+1, f) == sum(i, j, f) + f(j+1) 
+  {
+     lem_sumDropLast(i, j, f);
+  }
+}
+
+// i <= j+1 ==> sum_{k=i}^{j}c = c*(j - i + 1)
+lemma lem_sumOverConst(i:int, j:int, c:int)
+  requires i <= j+1
+  ensures sum(i, j, k => c) == c*(j - i + 1)
+{ 
+  var fr := liftCi2r(k => c);
+  var c' := c as real;
+  assert c' == c as real;
+  lem_sumrOverConst(i, j, c');
+  assert sumr(i, j, k => c') == (c*(j - i + 1)) as real;
+  lem_sum_liftCi2r_eq(i, j, k => c);
+  assert sumr(i, j, fr) == sum(i, j, k => c) as real;
+  assert sumr(i, j, fr) == sumr(i, j, k => c')
+   by { assert forall k:int :: i<=k<=j ==> c as real == c';
+        lem_sumrLeibniz(i, j, fr, k => c'); } 
+} 
+
+lemma lem_sumOverConstAll(i:int, j:int)
+  requires i <= j+1
+  ensures forall c:int :: sum(i, j, k => c) == (c*(j - i + 1))
+{ 
+  forall c:int
+    ensures sum(i, j, k => c) == (c*(j - i + 1))
   {
      lem_sumOverConst(i, j, c);
   }
 } 
 
-// i <= j+1 ==> sum_{k=i}^{j}k = (j*(j+1) + i*(1-i))/2 
-lemma lem_sumInterval(i:nat, j:nat)
+// i <= j+1 /\ (∀ k : i<=k<=j : f(k) == g(k)) 
+//          ==> sum_{k=i}^{j}f = sum_{k=i}^{j}g
+lemma {:axiom} lem_sumLeibniz(i:int, j:int, f:int->int, g:int->int)
   requires i <= j+1
+  requires forall k:int :: i<=k<=j ==> f(k) == g(k)
+  ensures sum(i, j, f) == sum(i, j, g)
+
+// Following sum lemmas are only stated for integers
+
+// i <= j+1 ==> sum_{k=i}^{j}k = (j*(j+1) + i*(1-i))/2 
+lemma lem_sumInterval(i:int, j:int)
+  requires i <= j+1 
   decreases j - i
-  ensures sum(i, j, k => k) == (j*(j+1) + i*(1-i))/2 
+  ensures sum(i, j, k => k) == (j*(j+1) + i*(1-i))/2
 { 
   if i == j+1 {   
     // BC: i > j
@@ -419,7 +498,7 @@ lemma lem_sumInterval(i:nat, j:nat)
       == { reveal sum(); }
          i + sum(i+1, j, k => k);
       == { lem_sumInterval(i+1, j); }  // by IH
-         i + (j*(j+1) + (i+1)*(1-(i+1)))/2 ;
+         i + (j*(j+1) + (i+1)*(1-(i+1)))/2;
       == 
          (j*(j+1) + i*(1-i))/2;            
     }
@@ -427,34 +506,27 @@ lemma lem_sumInterval(i:nat, j:nat)
 }
 
 // sum_{k=1}^{n}k = (n*(n+1))/2 
-lemma lem_sumGauss(n:nat)
-  ensures sum(1, n, k => k) == (n*(n+1))/2 
+lemma lem_sumTriangle(n:nat)
+  ensures sum(1, n, k => k) == (n*(n+1))/2
 {
-   lem_sumInterval(1, n);
+  lem_sumInterval(1, n);
 }
 
-// i <= j+1 /\ (∀ k : i<=k<=j : f(k) == g(k)) 
-//          ==> sum_{k=i}^{j}f = sum_{k=i}^{j}g
-lemma {:axiom} lem_sumLeibniz(i:nat, j:nat, f:nat->nat, g:nat->nat)
-  requires i <= j+1
-  requires forall k:nat :: i<=k<=j ==> f(k) == g(k)
-  ensures sum(i, j, f) == sum(i, j, g)
-
 // i <= j+1 ==> sum_{k=i}^{j}(j-k+i) = sum_{k=i}^{j}k
-lemma {:axiom} lem_sumReverseIndex(i:nat, j:nat)
+lemma {:axiom} lem_sumReverseIndex(i:int, j:int)
   requires i <= j+1
-  ensures sum(i, j, k => if i<=k<=j then j-k+i else 0) == sum(i, j, k => k)
+  ensures sum(i, j, k => j-k+i) == sum(i, j, k => k)
 
 
 /**************************************************************************
   Sum over sequences
 **************************************************************************/
 
-ghost function sumSeq(s:seq<nat>, f:nat->nat): nat
+opaque ghost function sumSeq(s:seq<int>, f:int->real): real
   decreases s
 {
   if |s| == 0 
-  then 0
+  then 0.0
   else f(s[0]) + sumSeq(s[1..], f)
 }
 
@@ -462,11 +534,11 @@ ghost function sumSeq(s:seq<nat>, f:nat->nat): nat
   Sum over sets
 **************************************************************************/
 
-ghost function sumSet(s:set<nat>, f:nat->nat): nat
+opaque ghost function sumSet(s:set<int>, f:int->real): real
   decreases s
 {
   if |s| == 0 
-  then 0
+  then 0.0
   else var x :| x in s;
        f(x) + sumSet(s - {x}, f)
 }
@@ -475,7 +547,23 @@ ghost function sumSet(s:set<nat>, f:nat->nat): nat
   Miscelanious stuff
 **************************************************************************/
 
-// no sirve pa un carajo
+ghost function liftD<T>(f:nat->T, default:T) : int->T
+{
+  k => if k < 0 then default else f(k as nat)
+}
+
+ghost function liftCi2r(f:int->int) : int->real
+{
+  n => f(n) as real
+}
+
+// Lift f:nat->nat to f':nat->R0
+ghost function liftToR0(f:nat->nat) : nat->R0
+{
+  n => f(n) as R0
+}
+
+// apparently useless
 ghost function ite<T>(cond: bool, thenBranch: T, elseBranch: T) : T
 {
   if cond then thenBranch else elseBranch
