analysisByMM/quad.dfy
@@ -62,7 +62,7 @@ lemma lem_T2def(n:nat)
 }
 
 lemma lem_T1BigOquad(N:nat)
-  ensures bigOR0(liftToR0(n => T1(n,N)), n => powr0(n as R0, 2.0))
+  ensures bigOR0(liftToR0(n => T1(n,N)), n => powr(n as R0, 2.0))
 {
   var a:nat       := 1;
   var b:nat       := 0;
@@ -74,18 +74,18 @@ lemma lem_T1BigOquad(N:nat)
 
   assert b >= s-1; 
   forall n:nat 
-    ensures T1'(n) == TbodyLR2(a, b, c, s, T1', w, k, n)
+    ensures T1'(n) == TbodyLR2(a, b, c, s, T1', w, n)
   {
     reveal TbodyLR2; 
     lem_T1def(n, N);
   } 
-  assert bigOR0(w, n => powr0(n as R0, k))
+  assert bigOR0(w, n => powr(n as R0, k))
    by { lem_T1BigOquadAux(N); }
   masterMethodLR2(a, b, c, s, T1', w, k); 
 }
 
 lemma {:isolate_assertions} lem_T1BigOquadAux(N:nat)
-  ensures bigOR0(liftToR0(n => T2(N)), n => powr0(n as R0, 1.0))
+  ensures bigOR0(liftToR0(n => T2(N)), n => powr(n as R0, 1.0))
 {
   var k:R0 := 1.0;
   var w:nat->R0 := liftToR0(n => T2(N)); 
@@ -93,21 +93,21 @@ lemma {:isolate_assertions} lem_T1BigOquadAux(N:nat)
   var c:R0 := T2(N) as R0;
   var n0:nat := 1; 
   forall n:nat | 0 <= 1 <= n
-    ensures w(n) <= c * powr0(n as R0, k) as R0
+    ensures w(n) <= c * powr(n as R0, k) as R0
   {
     assert T2(N) as R0 <= c * n as R0
       by { assert T2(N) <= (T2(N))*n; }
-    assert powr0(n as R0, k) == n as R0 
+    assert powr(n as R0, k) == n as R0 
       by { assert n as R0 > 0.0; lem_powrOne(n as R0); }
-    assert T2(N) as R0 <= c * powr0(n as R0, k); 
-    assert w(n) <= c * powr0(n as R0, k)
+    assert T2(N) as R0 <= c * powr(n as R0, k); 
+    assert w(n) <= c * powr(n as R0, k)
       by { assert w(n) == T2(N) as R0; }
   }
-  assert bigOR0from(c, n0, w, n => powr0(n as R0, k));  
+  assert bigOR0from(c, n0, w, n => powr(n as R0, k));  
 }
 
 lemma lem_T2BigOlin()
-  ensures bigOR0(liftToR0(T2), n => powr0(n as R0, 1.0))
+  ensures bigOR0(liftToR0(T2), n => powr(n as R0, 1.0))
 {
   var a:nat       := 1;
   var b:nat       := 0;
@@ -118,17 +118,17 @@ lemma lem_T2BigOlin()
   var w:nat->R0   := liftToR0(n => 1);
 
   forall n:nat 
-    ensures T2'(n) == TbodyLR2(a, b, c, s, T2', w, k, n)
+    ensures T2'(n) == TbodyLR2(a, b, c, s, T2', w, n)
   {
     reveal TbodyLR2;
     lem_T2def(n);
   } 
-  assert bigOR0(w, n => powr0(n as R0, k)) by {   
+  assert bigOR0(w, n => powr(n as R0, k)) by {   
     // we show that c=1 and n0=1
     forall n:nat | 0 <= 1 <= n
       ensures w(n) <= 1.0*polyGrowthR0(k)(n)
     {
-      assert powr0(n as R0, k) == 1.0 by { lem_powrZeroAll(); }
+      assert powr(n as R0, k) == 1.0 by { lem_powrZeroAll(); }
       assert w(n) <= 1.0*polyGrowthR0(k)(n); 
     }
     assert bigOR0from(1.0, 1, w, polyGrowthR0(k));
