test/testMath.dfy
@@ -1,6 +1,12 @@
 
 include "../theory/math.dfy"
 
+ghost method test_sumrInterval() {
+  reveal sumr();
+  var s := sumr(0, 2, x => 1.0);
+  assert s == 3.0; 
+}
+
 ghost method test_sumInterval() {
   reveal sum();
   var s := sum(0, 2, x => 1);
@@ -8,11 +14,13 @@ ghost method test_sumInterval() {
 }
 
 ghost method test_sumSeq() {
-  var s := sumSeq([0,1,2], x => 1);
-  assert s == 3; 
+  reveal sumSeq();
+  var s := sumSeq([0,1,2], x => 1.0);
+  assert s == 3.0; 
 }
-
+ 
 ghost method test_sumSet() {
-  var s2 := sumSet({0,1,2}, x => 1);
-  // assert s2 == 3; // no funciona
-} 
+  reveal sumSet();
+  var s2 := sumSet({0,1,2}, x => 1.0);
+  // assert s2 == 3.0;  // not working
+}
